Distinguish [long] and [long long]

theories/lang/cpp/arith/types.v
@@ -8,78 +8,6 @@ Require Import bedrock.prelude.base.
 
 #[local] Open Scope Z_scope.
 
-(* Bit-widths *)
-Variant bitsize : Set :=
-| W8
-| W16
-| W32
-| W64
-| W128.
-#[global] Instance bitsize_eq: EqDecision bitsize.
-Proof. solve_decision. Defined.
-#[global] Instance bitsize_countable : Countable bitsize.
-Proof.
-  apply (inj_countable'
-    (λ b,
-      match b with
-      | W8 => 0 | W16 => 1 | W32 => 2 | W64 => 3 | W128 => 4
-      end)
-    (λ n,
-      match n with
-      | 0 => W8 | 1 => W16 | 2 => W32 | 3 => W64 | 4 => W128
-      | _ => W8	(* dummy *)
-      end)).
-  abstract (by intros []).
-Defined.
-
-Definition bitsN (s : bitsize) : N :=
-  match s with
-  | W8   => 8
-  | W16  => 16
-  | W32  => 32
-  | W64  => 64
-  | W128 => 128
-  end.
-
-#[global] Instance bitsN_inj : Inj (=) (=) bitsN.
-Proof. red; intros x y H; by (destruct x; destruct y). Qed.
-
-Definition bitsZ (s : bitsize) : Z :=
-  Z.of_N (bitsN s).
-
-Definition bytesNat (s : bitsize) : nat :=
-  match s with
-  | W8 => 1
-  | W16 => 2
-  | W32 => 4
-  | W64 => 8
-  | W128 => 16
-  end.
-
-Definition bytesN (s : bitsize) : N :=
-  N.of_nat (bytesNat s).
-
-Definition bytesZ (s : bitsize) : Z :=
-  Z.of_N (bytesN s).
-
-#[global] Arguments N.of_nat !_ /.
-#[global] Arguments bytesN !_ /.
-#[global] Arguments bytesZ !_ /.
-
-Bind Scope N_scope with bitsize.
-
-Lemma of_size_gt_O w :
-  (0 < 2 ^ bitsZ w)%Z.
-Proof. destruct w; reflexivity. Qed.
-(* Hint Resolve of_size_gt_O. *)
-
-Lemma bytesZ_positive s :
-  (0 < bytesZ s)%Z.
-Proof. destruct s; reflexivity. Qed.
-
-Lemma bytesZ_range s : (0 < bytesZ s < 17)%Z.
-Proof. destruct s; cbn; lia. Qed.
-
 (* Signed and Unsigned *)
 Variant signed : Set := Signed | Unsigned.
 #[global] Instance signed_eq_dec: EqDecision signed.
@@ -87,41 +15,111 @@ Proof. solve_decision. Defined.
 #[global] Instance signed_countable : Countable signed.
 Proof.
   apply (inj_countable'
-    (λ s, if s is Signed then true else false)
-    (λ b, if b then Signed else Unsigned)).
+           (λ s, if s is Signed then true else false)
+           (λ b, if b then Signed else Unsigned)).
   abstract (by intros []).
 Defined.
+
+(* These take a bitsize in [N] *)
+Definition bits_min_val (n : N) (sgn : signed) : Z :=
+  match sgn with
+  | Signed => -(2^(Z.of_N n - 1))
+  | Unsigned => 0
+  end.
+Definition bits_max_val (n : N) (sgn : signed) : Z :=
+  match sgn with
+  | Signed => 2^(Z.of_N n-1) - 1
+  | Unsigned => 2^(Z.of_N n) - 1
+  end.
+Definition bits_bound n sgn (z : Z) : Prop :=
+  bits_min_val n sgn <= z <= bits_max_val n sgn.
+
+
+(* Bit-widths *)
+Module bitsize.
+  Variant t : Set :=
+  | W8
+  | W16
+  | W32
+  | W64
+  | W128.
+  Notation bitsize := t.
+  #[global] Instance bitsize_eq: EqDecision bitsize.
+  Proof. solve_decision. Defined.
+  #[global] Instance bitsize_countable : Countable bitsize.
+  Proof.
+    apply (inj_countable'
+      (λ b,
+        match b with
+        | W8 => 0 | W16 => 1 | W32 => 2 | W64 => 3 | W128 => 4
+        end)
+      (λ n,
+        match n with
+        | 0 => W8 | 1 => W16 | 2 => W32 | 3 => W64 | 4 => W128
+        | _ => W8	(* dummy *)
+        end)).
+    abstract (by intros []).
+  Defined.
+
+  Definition bitsN (s : bitsize) : N :=
+    match s with
+    | W8   => 8
+    | W16  => 16
+    | W32  => 32
+    | W64  => 64
+    | W128 => 128
+    end.
+
+  #[global] Instance bitsN_inj : Inj (=) (=) bitsN.
+  Proof. red; intros x y H; by (destruct x; destruct y). Qed.
+
+  Definition bitsZ (s : bitsize) : Z :=
+    Z.of_N (bitsN s).
+
+  Definition bytesNat (s : bitsize) : nat :=
+    match s with
+    | W8 => 1
+    | W16 => 2
+    | W32 => 4
+    | W64 => 8
+    | W128 => 16
+    end.
+
+  Definition bytesN (s : bitsize) : N :=
+    N.of_nat (bytesNat s).
+
+  Definition bytesZ (s : bitsize) : Z :=
+    Z.of_N (bytesN s).
+
+  Definition max_val (bits : bitsize) (sgn : signed) : Z :=
+    bits_max_val (bitsN bits) sgn.
+
+  Definition min_val (bits : bitsize) (sgn : signed) : Z :=
+    bits_min_val (bitsN bits) sgn.
+
+  Definition bound (bits : bitsize) (sgn : signed) (v : Z) : Prop :=
+    min_val bits sgn <= v <= max_val bits sgn.
+
+End bitsize.
+Notation bitsize := bitsize.t.
+#[global] Arguments N.of_nat !_ /.
+#[global] Arguments bitsize.bytesN !_ /.
+#[global] Arguments bitsize.bytesZ !_ /.
+
+Bind Scope N_scope with bitsize.
+
+Lemma of_size_gt_O w :
+  (0 < 2 ^ bitsize.bitsZ w)%Z.
+Proof. destruct w; reflexivity. Qed.
+(* Hint Resolve of_size_gt_O. *)
+
+Lemma bytesZ_positive s :
+  (0 < bitsize.bytesZ s)%Z.
+Proof. destruct s; reflexivity. Qed.
+
+Lemma bytesZ_range s : (0 < bitsize.bytesZ s < 17)%Z.
+Proof. destruct s; cbn; lia. Qed.
 
 Variant endian : Set := Little | Big.
 #[global] Instance endian_dec : EqDecision endian.
 Proof. solve_decision. Defined.
-
-Definition max_val (bits : bitsize) (sgn : signed) : Z :=
-  match bits , sgn with
-  | W8   , Signed   => 2^7 - 1
-  | W8   , Unsigned => 2^8 - 1
-  | W16  , Signed   => 2^15 - 1
-  | W16  , Unsigned => 2^16 - 1
-  | W32  , Signed   => 2^31 - 1
-  | W32  , Unsigned => 2^32 - 1
-  | W64  , Signed   => 2^63 - 1
-  | W64  , Unsigned => 2^64 - 1
-  | W128 , Signed   => 2^127 - 1
-  | W128 , Unsigned => 2^128 - 1
-  end.
-
-Definition min_val (bits : bitsize) (sgn : signed) : Z :=
-  match sgn with
-  | Unsigned => 0
-  | Signed =>
-    match bits with
-    | W8   => -2^7
-    | W16  => -2^15
-    | W32  => -2^31
-    | W64  => -2^63
-    | W128 => -2^127
-    end
-  end.
-
-Definition bound (bits : bitsize) (sgn : signed) (v : Z) : Prop :=
-  min_val bits sgn <= v <= max_val bits sgn.
