theories/lang/cpp/semantics/types.v
@@ -16,7 +16,7 @@ Definition GlobDecl_size_of (g : GlobDecl) : option N :=
   | Genum t _ =>
     match drop_qualifiers t with
     | Tchar_ sz => Some $ char_type.bytesN sz
-    | Tnum sz _ => Some $ bytesN sz
+    | Tnum sz _ => Some $ int_rank.bytesN sz
     | Tbool => Some 1%N
     | _ => None
     end
@@ -29,7 +29,7 @@ Definition GlobDecl_align_of (g : GlobDecl) : option N :=
   | Genum t _ =>
     match drop_qualifiers t with
     | Tchar_ sz => Some $ char_type.bytesN sz
-    | Tnum sz _ => Some $ bytesN sz
+    | Tnum sz _ => Some $ int_rank.bytesN sz
     | Tbool => Some 1%N
     | _ => None
     end
@@ -68,7 +68,7 @@ Fixpoint size_of (resolve : genv) (t : type) : option N :=
   | Tptr _ => Some (pointer_size resolve)
   | Tref _ => None
   | Trv_ref _ => None
-  | Tnum sz _ => Some (bytesN sz)
+  | Tnum sz _ => Some (int_rank.bytesN sz)
   | Tchar_ ct => Some (char_type.bytesN ct)
   | Tvoid => None
   | Tarray t n => N.mul n <$> size_of resolve t
@@ -82,7 +82,7 @@ Fixpoint size_of (resolve : genv) (t : type) : option N :=
   | Tqualified _ t => size_of resolve t
   | Tnullptr => Some (pointer_size resolve)
   | Tfloat_ sz => Some (float_type.bytesN sz)
-  | Tarch sz _ => bytesN <$> sz
+  | Tarch sz _ => bitsize.bytesN <$> sz
   | Tunsupported _ => None
   | Tdecltype _
   | Texprtype _
@@ -98,10 +98,10 @@ Fixpoint size_of (resolve : genv) (t : type) : option N :=
   end%N.
 
 (* [size_of] result can overflow: *)
-Goal forall σ, size_of σ (Tarray Tu8 (2^128)) = Some (2^128)%N.
+Goal forall σ, size_of σ (Tarray Tchar (2^128)) = Some (2^128)%N.
 Proof. by []. Abort.
 (* [size_of] result can overflow, even with in-bounds arguments: *)
-Goal forall σ, size_of σ (Tarray Tu64 (2^61)) = Some (2^64)%N.
+Goal forall σ, size_of σ (Tarray Tlonglong (2^61)) = Some (2^64)%N.
 Proof. by []. Abort.
 
 #[global] Instance Proper_size_of
@@ -110,7 +110,7 @@ Proof.
   intros ?? Hle ? t ->; induction t; simpl; (try constructor) => //.
   all: try exact: pointer_size_proper.
   - by destruct IHt; constructor; subst.
-  - rewrite /glob_def.
+(*  - rewrite /glob_def.
     generalize (types_compat _ _ (tu_le Hle) gn).
     destruct (types (genv_tu x) !! gn) eqn:Heq; simpl.
     { intro H; destruct (H _ Heq) as [?[Heq' ?]].
@@ -124,11 +124,22 @@ Proof.
       rewrite Heq' /=.
       by eapply proper_GlobDecl_size_of. }
     { intros. constructor. }
+*)
+  - rewrite /glob_def. move: Hle => [[ /(_ gn) Hle _] _ _].
+    revert Hle.
+    case: (types (genv_tu x) !! gn); simpl; try constructor.
+    move => ? /(_ _ eq_refl) [g2 [-> HH]] /=.
+    exact: proper_GlobDecl_size_of.
+  - rewrite /glob_def. move: Hle => [[ /(_ gn) Hle _] _ _].
+    revert Hle.
+    case: (types (genv_tu x) !! gn); simpl; try constructor.
+    move => ? /(_ _ eq_refl) [g2 [-> HH]] /=.
+    exact: proper_GlobDecl_size_of.
   - by destruct osz; constructor.
 Qed.
 
 Theorem size_of_int : forall {c : genv} s w,
-    @size_of c (Tnum w s) = Some (bytesN w).
+    @size_of c (Tnum w s) = Some (int_rank.bytesN w).
 Proof. reflexivity. Qed.
 Theorem size_of_char : forall {c : genv} s,
     @size_of c (Tchar_ s) = Some (char_type.bytesN s).
@@ -240,7 +251,7 @@ Proof. done. Qed.
 
 (* TODO?: consider using [SizeOf (Tnum sz sgn) (bytesN sz)]. *)
 #[global] Instance int_size_of {σ : genv} sz sgn n :
-  TCEq (bytesN sz) n -> SizeOf (Tnum sz sgn) n.
+  TCEq (int_rank.bytesN sz) n -> SizeOf (Tnum sz sgn) n.
 Proof. by rewrite /SizeOf TCEq_eq=><-. Qed.
 
 (* TODO?: consider using [SizeOf (Tnum sz sgn) (char_type.bytesN ct)]. *)
@@ -257,7 +268,7 @@ Proof. done. Qed.
 Proof. by rewrite /SizeOf TCEq_eq=><-. Qed.
 
 #[global] Instance arch_size_of {σ : genv} sz name n :
-  TCEq (bytesN sz) n -> SizeOf (Tarch (Some sz) name) n.
+  TCEq (bitsize.bytesN sz) n -> SizeOf (Tarch (Some sz) name) n.
 Proof. by rewrite /SizeOf TCEq_eq=><-. Qed.
 
 (** [HasSize ty] means that C++ type [ty] has a defined size *)
