tests/ref_collapse.t/test.v
@@ -7,7 +7,7 @@
 Require Import bedrock.prelude.prelude.
 Require Import bedrock.lang.cpp.syntax.types.
 
-Notation T := (Tnum (lang:=lang.cpp) W32 Signed).
+Notation T := (Tnum (lang:=lang.cpp) int_rank.Iint Signed).
 Notation C := (tqualified (lang:=lang.cpp) QC) (only parsing).
 Notation V := (tqualified (lang:=lang.cpp) QV) (only parsing).
 Notation L := (tref (lang:=lang.cpp) QM) (only parsing).
