theories/lang/cpp/logic/z_to_bytes.v
@@ -10,51 +10,55 @@ Require Import stdpp.numbers.
 Require Import bedrock.lang.cpp.arith.types.
 Require Import bedrock.lang.cpp.semantics.values.
 
+Lemma N_of_nat_to_nat a b : N.of_nat a = b -> a = N.to_nat b.
+Proof. intros. lia. Qed.
+
 Section with_σ.
   Context {σ : genv}.
 
   Lemma _Z_to_bytes_has_type_prop (cnt : nat) (endianness : endian) sign (z : Z) :
-    List.Forall (fun (v : N) => has_type_prop (Vn v) Tu8) (_Z_to_bytes cnt endianness sign z).
+    List.Forall (fun (v : N) => has_type_prop (Vn v) Tbyte) (_Z_to_bytes cnt endianness sign z).
   Proof.
     eapply List.Forall_impl.
     2: { exact: _Z_to_bytes_range. }
     move => ? /= ?.
     rewrite -has_int_type.
-    rewrite/bound/min_val/max_val.
+    rewrite/bitsize.bound/bitsize.min_val/bitsize.max_val/=.
     lia.
   Qed.
 
-  Lemma _Z_from_bytes_unsigned_le_has_type_prop (sz : int_type.t) :
+  Lemma _Z_from_bytes_unsigned_le_has_type_prop (sz : int_rank.t) :
     forall (bytes : list N),
-      lengthN bytes = bytesN sz ->
+      lengthN bytes = int_rank.bytesN sz ->
       has_type_prop (_Z_from_bytes_unsigned_le bytes) (Tnum sz Unsigned).
   Proof.
-    intros * Hlength; rewrite -has_int_type/bound/=.
-    rewrite /lengthN/bytesN in Hlength; apply Nat2N.inj in Hlength.
+    intros * Hlength; rewrite -has_int_type/bitsize.bound/=.
+    rewrite /lengthN/int_rank.bytesN in Hlength.
+    apply N_of_nat_to_nat in Hlength.
     eapply _Z_from_bytes_unsigned_le_bound; rewrite Hlength.
     destruct sz=> /=; lia.
   Qed.
 
-  Lemma _Z_from_bytes_le_has_type_prop (bytes : list N) (sz : int_type.t) (sgn : signed) :
-    lengthN bytes = bytesN sz ->
+  Lemma _Z_from_bytes_le_has_type_prop (bytes : list N) (sz : int_rank.t) (sgn : signed) :
+    lengthN bytes = int_rank.bytesN sz ->
     has_type_prop (_Z_from_bytes_le sgn bytes) (Tnum sz sgn).
   Proof.
     move => Hlength. rewrite /_Z_from_bytes_le.
     case_match; subst; last by apply _Z_from_bytes_unsigned_le_has_type_prop.
-    rewrite /lengthN /bytesN in Hlength; apply Nat2N.inj in Hlength; rewrite Hlength.
+    rewrite /lengthN /int_rank.bytesN in Hlength. apply N_of_nat_to_nat in Hlength; rewrite Hlength.
     unfold operator.to_signed_bits.
     rewrite bool_decide_false; last by destruct sz.
     destruct sz => /=.
     all: repeat (destruct bytes as [|? bytes]; simpl in Hlength; try lia; clear Hlength).
-    all: case_bool_decide; rewrite -has_int_type /bound/=;
+    all: case_bool_decide; rewrite -has_int_type /bitsize.bound/=;
       try match goal with
       | |- context[Z.modulo ?a ?b] => pose proof (Z.mod_pos_bound a b ltac:(lia)); lia
       end.
   Qed.
 
   Lemma _Z_from_bytes_has_type_prop :
-    forall (endianness : endian) (sz : int_type.t) (sgn : signed) (bytes : list N),
-      lengthN bytes = bytesN sz ->
+    forall (endianness : endian) (sz : int_rank.t) (sgn : signed) (bytes : list N),
+      lengthN bytes = int_rank.bytesN sz ->
       has_type_prop (Vint (_Z_from_bytes endianness sgn bytes)) (Tnum sz sgn).
   Proof.
     intros * Hlength.
