theories/lang/cpp/semantics/genv.v
@@ -51,12 +51,12 @@ Record genv : Type :=
 Existing Class genv.
 Definition genv_byte_order (g : genv) : endian :=
   g.(genv_tu).(byte_order).
-Definition pointer_size (g : genv) := bytesN (pointer_size_bitsize g).
+Definition pointer_size (g : genv) := bitsize.bytesN (pointer_size_bitsize g).
 Definition genv_type_table (g : genv) : type_table :=
   g.(genv_tu).(types).
 
 Module integral_type.
-  Record t : Set := mk { size : int_type.t ; signedness : signed }.
+  Record t : Set := mk { size : int_rank.t ; signedness : signed }.
   Coercion to_type {lang} (v : t) : type' lang :=
     Tnum v.(size) v.(signedness).
 End integral_type.
@@ -72,19 +72,30 @@ Definition signedness_of_char (σ : genv) (ct : char_type) : signed :=
 (** [equivalent_int_type g ct] is the integral type that is equivalent
     (in rank and signedness) of [ct].
  *)
+#[local] Definition find_equiv (ct : char_type)
+  (res := find (fun a => bool_decide (char_type.bitsN ct <= int_rank.bitsN a)%N) int_rank.ranks)
+  : match res with
+    | None => unit
+    | Some _ => int_rank.t
+    end :=
+  match res as X return match X with
+                        | None => unit
+                        | Some _ => int_rank.t
+                        end with
+  | None => tt
+  | Some x => x
+  end.
+
 Definition equivalent_int_type (g : genv) (ct : char_type) : integral_type.t :=
   let bits :=
+    (* NOTE the setup here computes the appropriate type given the size
+       constraints defined in [char_type.bitsN] and [int_type.bitsN] *)
     match ct with
-    | char_type.Cchar => int_type.Ichar
-    | _ =>
-        match char_type.bitsN ct with
-        | 8 => W8
-        | 16 => W16
-        | 32 => W32
-        | 64 => W64
-        | 128 => W128
-        | _ => W8
-        end%N
+    | char_type.Cchar => int_rank.Ichar
+    | char_type.C8 => Evaluate (find_equiv char_type.C8)
+    | char_type.C16 => Evaluate (find_equiv char_type.C16)
+    | char_type.C32 => Evaluate (find_equiv char_type.C32)
+    | char_type.Cwchar => Evaluate (find_equiv char_type.Cwchar)
     end
   in
   integral_type.mk bits (signedness_of_char g ct).
