theories/noimport/doc/cpp/logic.v
@@ -70,7 +70,6 @@ Example e_int : Rep := intR q z. (** similarly, [sintR] and [uingR] *)
 Example e_short : Rep := shortR q z. (** similarly, [ushortR] and [sshortR] *)
 Example e_long : Rep := longR q z. (** similarly, [ulongR] and [slongR] *)
 Example e_longlong : Rep := longlongR q z. (** similarly, [ulonglongR] and [slonglongR] *)
-Example e_i8 : Rep := i8R q z. (** similarly, [int16], [int32], [uint64]. Prefix 'u' for the unsigned variants *)
 
 (** Character types work a little bit differently because they are represented
     in an architecture-indepenent way as *unsigned* numbers *)
@@ -99,8 +98,8 @@ Example eptr : Rep := ptrR<ctype> q p.
 [ctype] is the C++ type of the pointer.
 Click at [type] to see the current definition of C++ types.
 For example, below, we are saying that the pointer is of type
-signed 64 bit (long * ) *)
-Example eptr2 : Rep := ptrR<Ti64> q p.
+<<long*>> *)
+Example eptr2 : Rep := ptrR<Tlong> q p.
 
 (**
 To refer to (named) struct types, use the [Tnamed] constructor,
@@ -108,7 +107,7 @@ which takes as argument the mangled name of the class/struct.
 We can use the notations defined in the names file to write
 unmangled names. More about this in the next chapters.
 *)
-Example eptr3 : Rep := ptrR<Tnamed (Nglobal $ Nid "list")> q p.
+Example eptr3 : Rep := ptrR<Tnamed "list"> q p.
 
 (** * Separation
 *)
